Kue/Json.lean
@@ -49,7 +49,7 @@ def manifestPrimToJson : Prim -> String
   | .bool true => "true"
   | .bool false => "false"
   | .int value => toString value
-  | .float value => value
+  | .float _ text => text
   | .string value => jsonString value
   | .bytes value => jsonString (base64Encode value.toList)
 
